<?xml version="1.0"?>
<rdf:RDF xmlns="http://www.semanticweb.org/leopo/ontologies/2022/0/EmergencyAgent#"
     xml:base="http://www.semanticweb.org/leopo/ontologies/2022/0/EmergencyAgent"
     xmlns:owl="http://www.w3.org/2002/07/owl#"
     xmlns:rdf="http://www.w3.org/1999/02/22-rdf-syntax-ns#"
     xmlns:xml="http://www.w3.org/XML/1998/namespace"
     xmlns:xsd="http://www.w3.org/2001/XMLSchema#"
     xmlns:rdfs="http://www.w3.org/2000/01/rdf-schema#">
    <owl:Ontology rdf:about="http://www.semanticweb.org/leopo/ontologies/2022/0/EmergencyAgent">
        <OWLAnnotationProperty_56383cae_6062_4e24_9cfb_5fb5b9e8c2b6code_license rdf:resource="https://spdx.org/licenses/MIT.html"/>
        <OWLAnnotationProperty_e51455f4_a5fc_4bb8_9c03_da23e0f3a39bcode_license xml:lang="en">The MIT License (MIT)

Copyright (c) 2022 Leopoldo Santos Santos of EmergencyAgent

Permission is hereby granted, free of charge, to any person obtaining a copy
of this software and associated documentation files (the &quot;Software&quot;), to deal
in the Software without restriction, including without limitation the rights
to use, copy, modify, merge, publish, distribute, sublicense, and/or sell
copies of the Software, and to permit persons to whom the Software is
furnished to do so, subject to the following conditions:

The above copyright notice and this permission notice shall be included in
all copies or substantial portions of the Software.

THE SOFTWARE IS PROVIDED &quot;AS IS&quot;, WITHOUT WARRANTY OF ANY KIND, EXPRESS OR
IMPLIED, INCLUDING BUT NOT LIMITED TO THE WARRANTIES OF MERCHANTABILITY,
FITNESS FOR A PARTICULAR PURPOSE AND NONINFRINGEMENT. IN NO EVENT SHALL THE
AUTHORS OR COPYRIGHT HOLDERS BE LIABLE FOR ANY CLAIM, DAMAGES OR OTHER
LIABILITY, WHETHER IN AN ACTION OF CONTRACT, TORT OR OTHERWISE, ARISING FROM,
OUT OF OR IN CONNECTION WITH THE SOFTWARE OR THE USE OR OTHER DEALINGS IN
THE SOFTWARE.</OWLAnnotationProperty_e51455f4_a5fc_4bb8_9c03_da23e0f3a39bcode_license>
        <rdfs:comment xml:lang="en">This ontology is designed to cover all  necessary personnel resources to manage an emergency situation.</rdfs:comment>
        <owl:versionInfo xml:lang="en">Version 1.0</owl:versionInfo>
    </owl:Ontology>
    


    <!-- 
    ///////////////////////////////////////////////////////////////////////////////////////
    //
    // Annotation properties
    //
    ///////////////////////////////////////////////////////////////////////////////////////
     -->

    


    <!-- http://www.semanticweb.org/leopo/ontologies/2022/0/EmergencyAgent#OWLAnnotationProperty_56383cae_6062_4e24_9cfb_5fb5b9e8c2b6code_license -->

    <owl:AnnotationProperty rdf:about="http://www.semanticweb.org/leopo/ontologies/2022/0/EmergencyAgent#OWLAnnotationProperty_56383cae_6062_4e24_9cfb_5fb5b9e8c2b6code_license">
        <rdfs:label xml:lang="es">code license</rdfs:label>
    </owl:AnnotationProperty>
    


    <!-- http://www.semanticweb.org/leopo/ontologies/2022/0/EmergencyAgent#OWLAnnotationProperty_e51455f4_a5fc_4bb8_9c03_da23e0f3a39bcode_license -->

    <owl:AnnotationProperty rdf:about="http://www.semanticweb.org/leopo/ontologies/2022/0/EmergencyAgent#OWLAnnotationProperty_e51455f4_a5fc_4bb8_9c03_da23e0f3a39bcode_license">
        <rdfs:label xml:lang="es">content license</rdfs:label>
    </owl:AnnotationProperty>
    


    <!-- 
    ///////////////////////////////////////////////////////////////////////////////////////
    //
    // Classes
    //
    ///////////////////////////////////////////////////////////////////////////////////////
     -->

    


    <!-- http://www.semanticweb.org/leopo/ontologies/2022/0/EmergencyAgent#AmbulanceDriverAgent -->

    <owl:Class rdf:about="http://www.semanticweb.org/leopo/ontologies/2022/0/EmergencyAgent#AmbulanceDriverAgent">
        <rdfs:subClassOf rdf:resource="http://www.semanticweb.org/leopo/ontologies/2022/0/EmergencyAgent#Volunteer"/>
        <rdfs:comment xml:lang="en">A person who has the right license and drives an ambulance</rdfs:comment>
    </owl:Class>
    


    <!-- http://www.semanticweb.org/leopo/ontologies/2022/0/EmergencyAgent#ArmedForcesBatallion -->

    <owl:Class rdf:about="http://www.semanticweb.org/leopo/ontologies/2022/0/EmergencyAgent#ArmedForcesBatallion">
        <rdfs:subClassOf rdf:resource="http://www.semanticweb.org/leopo/ontologies/2022/0/EmergencyAgent#ArmedForcesUnit"/>
        <rdfs:comment xml:lang="en">A tactical military organization composed basically of a headquarters and two or more companies, batteries, or similar organizations and usually commanded by a Lieutenant Colonel. Batallions can range from 500 to 600 troops (depending on the country).</rdfs:comment>
    </owl:Class>
    


    <!-- http://www.semanticweb.org/leopo/ontologies/2022/0/EmergencyAgent#ArmedForcesBrigade -->

    <owl:Class rdf:about="http://www.semanticweb.org/leopo/ontologies/2022/0/EmergencyAgent#ArmedForcesBrigade">
        <rdfs:subClassOf rdf:resource="http://www.semanticweb.org/leopo/ontologies/2022/0/EmergencyAgent#ArmedForcesUnit"/>
        <rdfs:comment xml:lang="en">A unit in military organization commanded by a brigadier general or colonel and composed of two or more subordinate units, such as regiments or battalions. Brigades can range from 3,000 to 5,000 troops depending on the country.</rdfs:comment>
    </owl:Class>
    


    <!-- http://www.semanticweb.org/leopo/ontologies/2022/0/EmergencyAgent#ArmedForcesCompany -->

    <owl:Class rdf:about="http://www.semanticweb.org/leopo/ontologies/2022/0/EmergencyAgent#ArmedForcesCompany">
        <rdfs:subClassOf rdf:resource="http://www.semanticweb.org/leopo/ontologies/2022/0/EmergencyAgent#ArmedForcesUnit"/>
        <rdfs:comment xml:lang="en">A Company is a body of soldiers that make up a unit (as of infantry) consisting usually of a headquarters and three platoons. It is commanded by a Captain.</rdfs:comment>
    </owl:Class>
    


    <!-- http://www.semanticweb.org/leopo/ontologies/2022/0/EmergencyAgent#ArmedForcesFireExtinguiserPlanePilot -->

    <owl:Class rdf:about="http://www.semanticweb.org/leopo/ontologies/2022/0/EmergencyAgent#ArmedForcesFireExtinguiserPlanePilot">
        <rdfs:subClassOf rdf:resource="http://www.semanticweb.org/leopo/ontologies/2022/0/EmergencyAgent#ArmedForcesUnit"/>
        <rdfs:comment xml:lang="en">A person who has a license to pilot aircraft and specialized in piloting firefighting aircraft.</rdfs:comment>
    </owl:Class>
    


    <!-- http://www.semanticweb.org/leopo/ontologies/2022/0/EmergencyAgent#ArmedForcesHelicopterPilot -->

    <owl:Class rdf:about="http://www.semanticweb.org/leopo/ontologies/2022/0/EmergencyAgent#ArmedForcesHelicopterPilot">
        <rdfs:subClassOf rdf:resource="http://www.semanticweb.org/leopo/ontologies/2022/0/EmergencyAgent#ArmedForcesUnit"/>
        <rdfs:comment xml:lang="en">A person who belong to Armed Forces and has a license to pilot a helicopter.</rdfs:comment>
    </owl:Class>
    


    <!-- http://www.semanticweb.org/leopo/ontologies/2022/0/EmergencyAgent#ArmedForcesPlatoon -->

    <owl:Class rdf:about="http://www.semanticweb.org/leopo/ontologies/2022/0/EmergencyAgent#ArmedForcesPlatoon">
        <rdfs:subClassOf rdf:resource="http://www.semanticweb.org/leopo/ontologies/2022/0/EmergencyAgent#ArmedForcesUnit"/>
        <rdfs:comment xml:lang="en">A Platoon is a body of soldiers that make up a unit (as of infantry) consisting usually of three squads. It is commanded by a Lieutenant.</rdfs:comment>
    </owl:Class>
    


    <!-- http://www.semanticweb.org/leopo/ontologies/2022/0/EmergencyAgent#ArmedForcesSquad -->

    <owl:Class rdf:about="http://www.semanticweb.org/leopo/ontologies/2022/0/EmergencyAgent#ArmedForcesSquad">
        <rdfs:subClassOf rdf:resource="http://www.semanticweb.org/leopo/ontologies/2022/0/EmergencyAgent#ArmedForcesUnit"/>
        <rdfs:comment xml:lang="en">A Squad is a body of soldiers that make up a unit (as of infantry) consisting usually of two teams. It is commanded by a Sargent or Sargent First Class.</rdfs:comment>
    </owl:Class>
    


    <!-- http://www.semanticweb.org/leopo/ontologies/2022/0/EmergencyAgent#ArmedForcesTeam -->

    <owl:Class rdf:about="http://www.semanticweb.org/leopo/ontologies/2022/0/EmergencyAgent#ArmedForcesTeam">
        <rdfs:subClassOf rdf:resource="http://www.semanticweb.org/leopo/ontologies/2022/0/EmergencyAgent#ArmedForcesUnit"/>
        <rdfs:comment xml:lang="en">A Team is a body of soldiers that make up a unit (as of infantry) consisting usually of four soldiers. It is commanded by a Corporal.</rdfs:comment>
    </owl:Class>
    


    <!-- http://www.semanticweb.org/leopo/ontologies/2022/0/EmergencyAgent#ArmedForcesUnit -->

    <owl:Class rdf:about="http://www.semanticweb.org/leopo/ontologies/2022/0/EmergencyAgent#ArmedForcesUnit">
        <rdfs:comment xml:lang="en">Armed Forces Unit represent all possible units that Armed Forces has.</rdfs:comment>
    </owl:Class>
    


    <!-- http://www.semanticweb.org/leopo/ontologies/2022/0/EmergencyAgent#BRIF-A -->

    <owl:Class rdf:about="http://www.semanticweb.org/leopo/ontologies/2022/0/EmergencyAgent#BRIF-A">
        <rdfs:subClassOf rdf:resource="http://www.semanticweb.org/leopo/ontologies/2022/0/EmergencyAgent#BRIFUnit"/>
        <rdfs:comment xml:lang="en">A BRIF-A Unit is a BRIF composed of about 60 people, and two helicopters</rdfs:comment>
    </owl:Class>
    


    <!-- http://www.semanticweb.org/leopo/ontologies/2022/0/EmergencyAgent#BRIF-B -->

    <owl:Class rdf:about="http://www.semanticweb.org/leopo/ontologies/2022/0/EmergencyAgent#BRIF-B">
        <rdfs:subClassOf rdf:resource="http://www.semanticweb.org/leopo/ontologies/2022/0/EmergencyAgent#BRIFUnit"/>
        <rdfs:comment xml:lang="en">A BRIF-B Unit is a BRIF composed of about 30 people, and one helicopter</rdfs:comment>
    </owl:Class>
    


    <!-- http://www.semanticweb.org/leopo/ontologies/2022/0/EmergencyAgent#BRIFUnit -->

    <owl:Class rdf:about="http://www.semanticweb.org/leopo/ontologies/2022/0/EmergencyAgent#BRIFUnit">
        <rdfs:comment xml:lang="en">BRIF means Reinforcement Brigades in Forest Fires. They are helicopter-borne units of highly specialized firefighting personnel. They provide a support service to the autonomous communities, being able to act at any point in the national territory, including the Canary Islands</rdfs:comment>
    </owl:Class>
    


    <!-- http://www.semanticweb.org/leopo/ontologies/2022/0/EmergencyAgent#BusDriverAgent -->

    <owl:Class rdf:about="http://www.semanticweb.org/leopo/ontologies/2022/0/EmergencyAgent#BusDriverAgent">
        <rdfs:subClassOf rdf:resource="http://www.semanticweb.org/leopo/ontologies/2022/0/EmergencyAgent#Volunteer"/>
        <rdfs:comment xml:lang="en">A bus driver is a driver with license to drive a bus.</rdfs:comment>
    </owl:Class>
    


    <!-- http://www.semanticweb.org/leopo/ontologies/2022/0/EmergencyAgent#CBRNAgent -->

    <owl:Class rdf:about="http://www.semanticweb.org/leopo/ontologies/2022/0/EmergencyAgent#CBRNAgent">
        <rdfs:subClassOf rdf:resource="http://www.semanticweb.org/leopo/ontologies/2022/0/EmergencyAgent#ArmedForcesUnit"/>
        <rdfs:comment xml:lang="en">A CBRN Agent is a person with training in CBRN. CBRN is an acronym for Chemical, Biological, Radiological and Nuclear.</rdfs:comment>
    </owl:Class>
    


    <!-- http://www.semanticweb.org/leopo/ontologies/2022/0/EmergencyAgent#CBRNArmedForcesAgent -->

    <owl:Class rdf:about="http://www.semanticweb.org/leopo/ontologies/2022/0/EmergencyAgent#CBRNArmedForcesAgent">
        <rdfs:subClassOf rdf:resource="http://www.semanticweb.org/leopo/ontologies/2022/0/EmergencyAgent#ArmedForcesUnit"/>
        <rdfs:comment xml:lang="en">A CBRN Armed Forces Agent is a person with training in CBRN who belongs to Armed Forces. CBRN is an acronym for Chemical, Biological, Radiological and Nuclear.</rdfs:comment>
    </owl:Class>
    


    <!-- http://www.semanticweb.org/leopo/ontologies/2022/0/EmergencyAgent#CBRNArmedForcesBatallion -->

    <owl:Class rdf:about="http://www.semanticweb.org/leopo/ontologies/2022/0/EmergencyAgent#CBRNArmedForcesBatallion">
        <rdfs:subClassOf rdf:resource="http://www.semanticweb.org/leopo/ontologies/2022/0/EmergencyAgent#ArmedForcesUnit"/>
        <rdfs:comment xml:lang="en">A tactical military organization, who belongs to Armed Forces and especialized in CBRN, composed basically of a headquarters and two or more companies, batteries, or similar organizations and usually commanded by a Lieutenant Colonel. Batallions can range from 500 to 600 troops (depending on the country).</rdfs:comment>
    </owl:Class>
    


    <!-- http://www.semanticweb.org/leopo/ontologies/2022/0/EmergencyAgent#CBRNArmedForcesCompany -->

    <owl:Class rdf:about="http://www.semanticweb.org/leopo/ontologies/2022/0/EmergencyAgent#CBRNArmedForcesCompany">
        <rdfs:subClassOf rdf:resource="http://www.semanticweb.org/leopo/ontologies/2022/0/EmergencyAgent#ArmedForcesUnit"/>
        <rdfs:comment xml:lang="en">A Company is a body of soldiers, who belongs to Armed Forces and especialized in CBRN, that make up a unit (as of infantry) consisting usually of a headquarters and three platoons. It is commanded by a Captain.</rdfs:comment>
    </owl:Class>
    


    <!-- http://www.semanticweb.org/leopo/ontologies/2022/0/EmergencyAgent#CBRNArmedForcesPlatoon -->

    <owl:Class rdf:about="http://www.semanticweb.org/leopo/ontologies/2022/0/EmergencyAgent#CBRNArmedForcesPlatoon">
        <rdfs:subClassOf rdf:resource="http://www.semanticweb.org/leopo/ontologies/2022/0/EmergencyAgent#ArmedForcesUnit"/>
        <rdfs:comment xml:lang="en">A Platoon is a body of soldiers, who belongs to Armed Forces and especialized in CBRN, that make up a unit (as of infantry) consisting usually of three squads. It is commanded by a Lieutenant.</rdfs:comment>
    </owl:Class>
    


    <!-- http://www.semanticweb.org/leopo/ontologies/2022/0/EmergencyAgent#CBRNArmedForcesSquad -->

    <owl:Class rdf:about="http://www.semanticweb.org/leopo/ontologies/2022/0/EmergencyAgent#CBRNArmedForcesSquad">
        <rdfs:subClassOf rdf:resource="http://www.semanticweb.org/leopo/ontologies/2022/0/EmergencyAgent#ArmedForcesUnit"/>
        <rdfs:comment xml:lang="en">A Squad is a body of soldiers, who belongs to Armed Forces and is especialized in CBRN, that make up a unit (as of infantry) consisting usually of two teams. It is commanded by a Sargent or Sargent First Class.</rdfs:comment>
    </owl:Class>
    


    <!-- http://www.semanticweb.org/leopo/ontologies/2022/0/EmergencyAgent#CBRNArmedForcesTeam -->

    <owl:Class rdf:about="http://www.semanticweb.org/leopo/ontologies/2022/0/EmergencyAgent#CBRNArmedForcesTeam">
        <rdfs:subClassOf rdf:resource="http://www.semanticweb.org/leopo/ontologies/2022/0/EmergencyAgent#ArmedForcesUnit"/>
        <rdfs:comment xml:lang="en">A Team is a body of soldiers, who belongs to Armed Forces ans is especialized in CBRN, that make up a unit (as of infantry) consisting usually of four soldiers. It is commanded by a Corporal.</rdfs:comment>
    </owl:Class>
    


    <!-- http://www.semanticweb.org/leopo/ontologies/2022/0/EmergencyAgent#CBRNUMEAgent -->

    <owl:Class rdf:about="http://www.semanticweb.org/leopo/ontologies/2022/0/EmergencyAgent#CBRNUMEAgent">
        <rdfs:subClassOf rdf:resource="http://www.semanticweb.org/leopo/ontologies/2022/0/EmergencyAgent#UMEUnit"/>
        <rdfs:comment xml:lang="en">A UME CBRN Agent is a person with training in CBRN who belongs to UME (Emergency Military Unit). CBRN is an acronym for Chemical, Biological, Radiological and Nuclear.</rdfs:comment>
    </owl:Class>
    


    <!-- http://www.semanticweb.org/leopo/ontologies/2022/0/EmergencyAgent#CBRNUMECompany -->

    <owl:Class rdf:about="http://www.semanticweb.org/leopo/ontologies/2022/0/EmergencyAgent#CBRNUMECompany">
        <rdfs:subClassOf rdf:resource="http://www.semanticweb.org/leopo/ontologies/2022/0/EmergencyAgent#UMEUnit"/>
        <rdfs:comment xml:lang="en">An CBRN UME Company is a body of soldiers, who belongs to UME and is especialized in CBRN, that make up a unit (as of infantry) consisting usually of a headquarters and three platoons. It is commanded by a Captain.</rdfs:comment>
    </owl:Class>
    


    <!-- http://www.semanticweb.org/leopo/ontologies/2022/0/EmergencyAgent#CBRNUMEPlatoon -->

    <owl:Class rdf:about="http://www.semanticweb.org/leopo/ontologies/2022/0/EmergencyAgent#CBRNUMEPlatoon">
        <rdfs:subClassOf rdf:resource="http://www.semanticweb.org/leopo/ontologies/2022/0/EmergencyAgent#UMEUnit"/>
        <rdfs:comment xml:lang="en">An CBRN UME Platoon is a body of soldiers, who belongs to UME and is especialized in CBRN, that make up a unit (as of infantry) consisting usually of three squads. It is commanded by a Lieutenant.</rdfs:comment>
    </owl:Class>
    


    <!-- http://www.semanticweb.org/leopo/ontologies/2022/0/EmergencyAgent#CBRNUMESquad -->

    <owl:Class rdf:about="http://www.semanticweb.org/leopo/ontologies/2022/0/EmergencyAgent#CBRNUMESquad">
        <rdfs:subClassOf rdf:resource="http://www.semanticweb.org/leopo/ontologies/2022/0/EmergencyAgent#UMEUnit"/>
        <rdfs:comment xml:lang="en">A CBRN UME Squad is a body of soldiers, who belongs to UME and is especialized in CBRN, that make up a unit (as of infantry) consisting usually of two teams. It is commanded by a Sargent or Sargent First Class.</rdfs:comment>
    </owl:Class>
    


    <!-- http://www.semanticweb.org/leopo/ontologies/2022/0/EmergencyAgent#CBRNUMETeam -->

    <owl:Class rdf:about="http://www.semanticweb.org/leopo/ontologies/2022/0/EmergencyAgent#CBRNUMETeam">
        <rdfs:subClassOf rdf:resource="http://www.semanticweb.org/leopo/ontologies/2022/0/EmergencyAgent#UMEUnit"/>
        <rdfs:comment xml:lang="en">A CBRN UME Team is a body of soldiers, who belongs to UME and is especialized in CBRN, that make up a unit (as of infantry) consisting usually of four soldiers. It is commanded by a Corporal.</rdfs:comment>
    </owl:Class>
    


    <!-- http://www.semanticweb.org/leopo/ontologies/2022/0/EmergencyAgent#CivilProtectionAgent -->

    <owl:Class rdf:about="http://www.semanticweb.org/leopo/ontologies/2022/0/EmergencyAgent#CivilProtectionAgent">
        <rdfs:subClassOf rdf:resource="http://www.semanticweb.org/leopo/ontologies/2022/0/EmergencyAgent#Volunteer"/>
        <rdfs:comment xml:lang="en">A Civil Protection Agent is a person who belongs to Civil Protection.</rdfs:comment>
    </owl:Class>
    


    <!-- http://www.semanticweb.org/leopo/ontologies/2022/0/EmergencyAgent#DoctorAgent -->

    <owl:Class rdf:about="http://www.semanticweb.org/leopo/ontologies/2022/0/EmergencyAgent#DoctorAgent">
        <rdfs:subClassOf rdf:resource="http://www.semanticweb.org/leopo/ontologies/2022/0/EmergencyAgent#MedicalServices"/>
        <owl:disjointWith rdf:resource="http://www.semanticweb.org/leopo/ontologies/2022/0/EmergencyAgent#HealthcareWorkerAgent"/>
        <owl:disjointWith rdf:resource="http://www.semanticweb.org/leopo/ontologies/2022/0/EmergencyAgent#PsychologistAgent"/>
        <rdfs:comment xml:lang="en">A person with a medical degree whose job is to treat people who are ill or hurt and who belongs to any kind of Units working in the Emergency.</rdfs:comment>
    </owl:Class>
    


    <!-- http://www.semanticweb.org/leopo/ontologies/2022/0/EmergencyAgent#FireBrigadeAgent -->

    <owl:Class rdf:about="http://www.semanticweb.org/leopo/ontologies/2022/0/EmergencyAgent#FireBrigadeAgent">
        <rdfs:subClassOf rdf:resource="http://www.semanticweb.org/leopo/ontologies/2022/0/EmergencyAgent#FireBrigadeUnit"/>
        <rdfs:comment xml:lang="en">A Fire Brigade Agent is a person with training in fire fighting and works in this field.</rdfs:comment>
    </owl:Class>
    


    <!-- http://www.semanticweb.org/leopo/ontologies/2022/0/EmergencyAgent#FireBrigadePlatoon -->

    <owl:Class rdf:about="http://www.semanticweb.org/leopo/ontologies/2022/0/EmergencyAgent#FireBrigadePlatoon">
        <rdfs:subClassOf rdf:resource="http://www.semanticweb.org/leopo/ontologies/2022/0/EmergencyAgent#FireBrigadeUnit"/>
        <rdfs:comment xml:lang="en">A Fire Fighting Platoon is a body of workers who has training in fire fighting and that make up a unit consisting usually of three squads.</rdfs:comment>
    </owl:Class>
    


    <!-- http://www.semanticweb.org/leopo/ontologies/2022/0/EmergencyAgent#FireBrigadeSquad -->

    <owl:Class rdf:about="http://www.semanticweb.org/leopo/ontologies/2022/0/EmergencyAgent#FireBrigadeSquad">
        <rdfs:subClassOf rdf:resource="http://www.semanticweb.org/leopo/ontologies/2022/0/EmergencyAgent#FireBrigadeUnit"/>
        <rdfs:comment xml:lang="en">A Fire Fighting Squad is a body of workers with training in fire fighting that make up a unit (as of infantry) consisting usually of two teams.</rdfs:comment>
    </owl:Class>
    


    <!-- http://www.semanticweb.org/leopo/ontologies/2022/0/EmergencyAgent#FireBrigadeTeam -->

    <owl:Class rdf:about="http://www.semanticweb.org/leopo/ontologies/2022/0/EmergencyAgent#FireBrigadeTeam">
        <rdfs:subClassOf rdf:resource="http://www.semanticweb.org/leopo/ontologies/2022/0/EmergencyAgent#FireBrigadeUnit"/>
        <rdfs:comment xml:lang="en">A Fire Fighting Team is a body of workers with trianing in fire fighting that make up a unit (as of infantry) consisting usually of four workers.</rdfs:comment>
    </owl:Class>
    


    <!-- http://www.semanticweb.org/leopo/ontologies/2022/0/EmergencyAgent#FireBrigadeUnit -->

    <owl:Class rdf:about="http://www.semanticweb.org/leopo/ontologies/2022/0/EmergencyAgent#FireBrigadeUnit">
        <rdfs:comment xml:lang="en">Fire Brigade Unit represent all possible units that regions contract to work in the fires.</rdfs:comment>
    </owl:Class>
    


    <!-- http://www.semanticweb.org/leopo/ontologies/2022/0/EmergencyAgent#GuardiaCivilAgent -->

    <owl:Class rdf:about="http://www.semanticweb.org/leopo/ontologies/2022/0/EmergencyAgent#GuardiaCivilAgent">
        <rdfs:subClassOf rdf:resource="http://www.semanticweb.org/leopo/ontologies/2022/0/EmergencyAgent#GuardiaCivilUnit"/>
        <rdfs:comment xml:lang="en">Is a person who belongs to Guardia Civil, which is a law enforcement force, a gendarmerie corps with a military nature with a permanent vocation for services.</rdfs:comment>
        <rdfs:isDefinedBy xml:lang="en">Is a person who belongs to Guardia Civil, which is a law enforcement force, a gendarmerie corps with a military nature with a permanent vocation for services.</rdfs:isDefinedBy>
    </owl:Class>
    


    <!-- http://www.semanticweb.org/leopo/ontologies/2022/0/EmergencyAgent#GuardiaCivilCompany -->

    <owl:Class rdf:about="http://www.semanticweb.org/leopo/ontologies/2022/0/EmergencyAgent#GuardiaCivilCompany">
        <rdfs:subClassOf rdf:resource="http://www.semanticweb.org/leopo/ontologies/2022/0/EmergencyAgent#GuardiaCivilUnit"/>
        <rdfs:comment xml:lang="en">A Guardia Civil Company is a body of Guardia Civil agents that make up a unit (as of infantry) consisting usually of a headquarters and three platoons. It is commanded by a Captain.</rdfs:comment>
        <rdfs:isDefinedBy xml:lang="en">A Guardia Civil Company is a body of Guardia Civil agents that make up a unit (as of infantry) consisting usually of a headquarters and three platoons. It is commanded by a Captain.</rdfs:isDefinedBy>
    </owl:Class>
    


    <!-- http://www.semanticweb.org/leopo/ontologies/2022/0/EmergencyAgent#GuardiaCivilPatrol -->

    <owl:Class rdf:about="http://www.semanticweb.org/leopo/ontologies/2022/0/EmergencyAgent#GuardiaCivilPatrol">
        <rdfs:subClassOf rdf:resource="http://www.semanticweb.org/leopo/ontologies/2022/0/EmergencyAgent#GuardiaCivilUnit"/>
        <rdfs:comment xml:lang="en">A Guardia Civil Patrol is a group of Guardia Civil agents, at least two of them.</rdfs:comment>
    </owl:Class>
    


    <!-- http://www.semanticweb.org/leopo/ontologies/2022/0/EmergencyAgent#GuardiaCivilPlatoon -->

    <owl:Class rdf:about="http://www.semanticweb.org/leopo/ontologies/2022/0/EmergencyAgent#GuardiaCivilPlatoon">
        <rdfs:subClassOf rdf:resource="http://www.semanticweb.org/leopo/ontologies/2022/0/EmergencyAgent#GuardiaCivilUnit"/>
        <rdfs:comment xml:lang="en">A Guardia Civil Platoon is a body of Guardia Civil agents, that make up a unit (as of infantry) consisting usually of three squads. It is commanded by a Lieutenant, or Second Lieutenant.</rdfs:comment>
    </owl:Class>
    


    <!-- http://www.semanticweb.org/leopo/ontologies/2022/0/EmergencyAgent#GuardiaCivilSquad -->

    <owl:Class rdf:about="http://www.semanticweb.org/leopo/ontologies/2022/0/EmergencyAgent#GuardiaCivilSquad">
        <rdfs:subClassOf rdf:resource="http://www.semanticweb.org/leopo/ontologies/2022/0/EmergencyAgent#GuardiaCivilUnit"/>
        <rdfs:comment xml:lang="en">A Guardi Civil Squad is a body of Guardia Civil agents that make up a unit (as of infantry) consisting usually of two teams. It is commanded by a Corporal First,  a Sargent or a Sargent First Class.</rdfs:comment>
    </owl:Class>
    


    <!-- http://www.semanticweb.org/leopo/ontologies/2022/0/EmergencyAgent#GuardiaCivilTeam -->

    <owl:Class rdf:about="http://www.semanticweb.org/leopo/ontologies/2022/0/EmergencyAgent#GuardiaCivilTeam">
        <rdfs:subClassOf rdf:resource="http://www.semanticweb.org/leopo/ontologies/2022/0/EmergencyAgent#GuardiaCivilUnit"/>
        <rdfs:comment xml:lang="en">A Guardia Civil Team is a body of Guardia Civil agents that make up a unit (as of infantry) consisting usually of two patrols . It is commanded by a Corporal.</rdfs:comment>
    </owl:Class>
    


    <!-- http://www.semanticweb.org/leopo/ontologies/2022/0/EmergencyAgent#GuardiaCivilUnit -->

    <owl:Class rdf:about="http://www.semanticweb.org/leopo/ontologies/2022/0/EmergencyAgent#GuardiaCivilUnit">
        <rdfs:comment xml:lang="en">Guardia Civil Unit represent all possible units that Guardia Civil have.</rdfs:comment>
        <rdfs:isDefinedBy xml:lang="en">Guardia Civil Unit represent all possible units that Guardia Civil have.</rdfs:isDefinedBy>
    </owl:Class>
    


    <!-- http://www.semanticweb.org/leopo/ontologies/2022/0/EmergencyAgent#HealthcareWorkerAgent -->

    <owl:Class rdf:about="http://www.semanticweb.org/leopo/ontologies/2022/0/EmergencyAgent#HealthcareWorkerAgent">
        <rdfs:subClassOf rdf:resource="http://www.semanticweb.org/leopo/ontologies/2022/0/EmergencyAgent#MedicalServices"/>
        <owl:disjointWith rdf:resource="http://www.semanticweb.org/leopo/ontologies/2022/0/EmergencyAgent#PsychologistAgent"/>
        <rdfs:comment xml:lang="en">A healthcare worker is anyone who works in a healthcare or social care setting, including healthcare students on clinical placement, frontline healthcare workers and other healthcare workers not in direct patient contact.</rdfs:comment>
    </owl:Class>
    


    <!-- http://www.semanticweb.org/leopo/ontologies/2022/0/EmergencyAgent#MedicalServices -->

    <owl:Class rdf:about="http://www.semanticweb.org/leopo/ontologies/2022/0/EmergencyAgent#MedicalServices">
        <rdfs:comment xml:lang="en">Medical services designed to urgently examine, care for, and treat injuries and wounds sustained during an emergency. These services are carried out, usually in a field hospital.</rdfs:comment>
    </owl:Class>
    


    <!-- http://www.semanticweb.org/leopo/ontologies/2022/0/EmergencyAgent#PoliceAgent -->

    <owl:Class rdf:about="http://www.semanticweb.org/leopo/ontologies/2022/0/EmergencyAgent#PoliceAgent">
        <rdfs:subClassOf rdf:resource="http://www.semanticweb.org/leopo/ontologies/2022/0/EmergencyAgent#PoliceUnit"/>
        <owl:disjointWith rdf:resource="http://www.semanticweb.org/leopo/ontologies/2022/0/EmergencyAgent#PolicePatrol"/>
        <rdfs:comment xml:lang="en">A person whose job is to enforce laws, investigate crimes, and make arrests: a member of the police.</rdfs:comment>
    </owl:Class>
    


    <!-- http://www.semanticweb.org/leopo/ontologies/2022/0/EmergencyAgent#PolicePatrol -->

    <owl:Class rdf:about="http://www.semanticweb.org/leopo/ontologies/2022/0/EmergencyAgent#PolicePatrol">
        <rdfs:subClassOf rdf:resource="http://www.semanticweb.org/leopo/ontologies/2022/0/EmergencyAgent#PoliceUnit"/>
        <rdfs:comment xml:lang="en">A Police Patrol is a group of Police agents, at least two of them.</rdfs:comment>
    </owl:Class>
    


    <!-- http://www.semanticweb.org/leopo/ontologies/2022/0/EmergencyAgent#PoliceUnit -->

    <owl:Class rdf:about="http://www.semanticweb.org/leopo/ontologies/2022/0/EmergencyAgent#PoliceUnit">
        <rdfs:comment xml:lang="en">Police Unit represent all possible units that Police have</rdfs:comment>
    </owl:Class>
    


    <!-- http://www.semanticweb.org/leopo/ontologies/2022/0/EmergencyAgent#PsychologistAgent -->

    <owl:Class rdf:about="http://www.semanticweb.org/leopo/ontologies/2022/0/EmergencyAgent#PsychologistAgent">
        <rdfs:subClassOf rdf:resource="http://www.semanticweb.org/leopo/ontologies/2022/0/EmergencyAgent#MedicalServices"/>
        <rdfs:comment xml:lang="en">An expert or specialist in psychology.</rdfs:comment>
    </owl:Class>
    


    <!-- http://www.semanticweb.org/leopo/ontologies/2022/0/EmergencyAgent#RedCrossAgent -->

    <owl:Class rdf:about="http://www.semanticweb.org/leopo/ontologies/2022/0/EmergencyAgent#RedCrossAgent">
        <rdfs:subClassOf rdf:resource="http://www.semanticweb.org/leopo/ontologies/2022/0/EmergencyAgent#Volunteer"/>
        <rdfs:comment xml:lang="en">A person who belongs to Red Cross. The Red Cross is an international organization that helps people who are suffering, for example as a result of war, floods, or disease.</rdfs:comment>
    </owl:Class>
    


    <!-- http://www.semanticweb.org/leopo/ontologies/2022/0/EmergencyAgent#RegionalEmergencyUnit -->

    <owl:Class rdf:about="http://www.semanticweb.org/leopo/ontologies/2022/0/EmergencyAgent#RegionalEmergencyUnit">
        <rdfs:comment xml:lang="en">It represents any kind of unit used by regions to work in emergencies like fires, floods, winter emergencies, etc.</rdfs:comment>
    </owl:Class>
    


    <!-- http://www.semanticweb.org/leopo/ontologies/2022/0/EmergencyAgent#SignalCorpsAgent -->

    <owl:Class rdf:about="http://www.semanticweb.org/leopo/ontologies/2022/0/EmergencyAgent#SignalCorpsAgent">
        <rdfs:subClassOf rdf:resource="http://www.semanticweb.org/leopo/ontologies/2022/0/EmergencyAgent#ArmedForcesUnit"/>
        <rdfs:comment xml:lang="en">A soldier who belongs to Signal Corps, which the part of an army in charge of communications.</rdfs:comment>
    </owl:Class>
    


    <!-- http://www.semanticweb.org/leopo/ontologies/2022/0/EmergencyAgent#SignalCorpsSquad -->

    <owl:Class rdf:about="http://www.semanticweb.org/leopo/ontologies/2022/0/EmergencyAgent#SignalCorpsSquad">
        <rdfs:subClassOf rdf:resource="http://www.semanticweb.org/leopo/ontologies/2022/0/EmergencyAgent#ArmedForcesUnit"/>
        <rdfs:comment xml:lang="en">A Squad is a body of soldiers, who belongs to Signal Corps,  that make up a unit (as of infantry) consisting usually of two teams. It is commanded by a Sargent or Sargent First Class.</rdfs:comment>
    </owl:Class>
    


    <!-- http://www.semanticweb.org/leopo/ontologies/2022/0/EmergencyAgent#SignalCorpsTeam -->

    <owl:Class rdf:about="http://www.semanticweb.org/leopo/ontologies/2022/0/EmergencyAgent#SignalCorpsTeam">
        <rdfs:subClassOf rdf:resource="http://www.semanticweb.org/leopo/ontologies/2022/0/EmergencyAgent#ArmedForcesUnit"/>
        <rdfs:comment xml:lang="en">A Signal Corps Team is a body of soldiers, who belongs to Signal Corps, that make up a unit (as of infantry) consisting usually of four soldiers. It is commanded by a Corporal.</rdfs:comment>
    </owl:Class>
    


    <!-- http://www.semanticweb.org/leopo/ontologies/2022/0/EmergencyAgent#TruckDriverAgent -->

    <owl:Class rdf:about="http://www.semanticweb.org/leopo/ontologies/2022/0/EmergencyAgent#TruckDriverAgent">
        <rdfs:subClassOf rdf:resource="http://www.semanticweb.org/leopo/ontologies/2022/0/EmergencyAgent#Volunteer"/>
        <rdfs:comment xml:lang="en">A person who has a driver licence to drive a truck</rdfs:comment>
    </owl:Class>
    


    <!-- http://www.semanticweb.org/leopo/ontologies/2022/0/EmergencyAgent#UMEBatallion -->

    <owl:Class rdf:about="http://www.semanticweb.org/leopo/ontologies/2022/0/EmergencyAgent#UMEBatallion">
        <rdfs:subClassOf rdf:resource="http://www.semanticweb.org/leopo/ontologies/2022/0/EmergencyAgent#UMEUnit"/>
        <rdfs:comment xml:lang="en">An UME Batallion is a tactical military organization, who belongs to UME (Emergency Military Unit), composed basically of a headquarters and two or more companies, batteries, or similar organizations and usually commanded by a Lieutenant Colonel. Batallions can range from 500 to 600 troops (depending on the country).</rdfs:comment>
    </owl:Class>
    


    <!-- http://www.semanticweb.org/leopo/ontologies/2022/0/EmergencyAgent#UMECompany -->

    <owl:Class rdf:about="http://www.semanticweb.org/leopo/ontologies/2022/0/EmergencyAgent#UMECompany">
        <rdfs:subClassOf rdf:resource="http://www.semanticweb.org/leopo/ontologies/2022/0/EmergencyAgent#UMEUnit"/>
        <rdfs:comment xml:lang="en">An UME Company is a body of soldiers, who belongs to UME (Emergency Military Unit), that make up a unit (as of infantry) consisting usually of a headquarters and three platoons. It is commanded by a Captain.</rdfs:comment>
    </owl:Class>
    


    <!-- http://www.semanticweb.org/leopo/ontologies/2022/0/EmergencyAgent#UMEPlatoon -->

    <owl:Class rdf:about="http://www.semanticweb.org/leopo/ontologies/2022/0/EmergencyAgent#UMEPlatoon">
        <rdfs:subClassOf rdf:resource="http://www.semanticweb.org/leopo/ontologies/2022/0/EmergencyAgent#UMEUnit"/>
        <rdfs:comment xml:lang="en">An UME Platoon is a body of soldiers, who belongs to UME (Emergency Military Unit) that make up a unit (as of infantry) consisting usually of three squads. It is commanded by a Lieutenant.</rdfs:comment>
    </owl:Class>
    


    <!-- http://www.semanticweb.org/leopo/ontologies/2022/0/EmergencyAgent#UMESoldierAgent -->

    <owl:Class rdf:about="http://www.semanticweb.org/leopo/ontologies/2022/0/EmergencyAgent#UMESoldierAgent">
        <rdfs:subClassOf rdf:resource="http://www.semanticweb.org/leopo/ontologies/2022/0/EmergencyAgent#UMEUnit"/>
        <rdfs:comment xml:lang="en">A UME Soldier is a person with training in different kind of emergencies who belongs to UME (Emergency Military Unit). CBRN is an acronym for Chemical, Biological, Radiological and Nuclear.</rdfs:comment>
    </owl:Class>
    


    <!-- http://www.semanticweb.org/leopo/ontologies/2022/0/EmergencyAgent#UMESquad -->

    <owl:Class rdf:about="http://www.semanticweb.org/leopo/ontologies/2022/0/EmergencyAgent#UMESquad">
        <rdfs:subClassOf rdf:resource="http://www.semanticweb.org/leopo/ontologies/2022/0/EmergencyAgent#UMEUnit"/>
        <rdfs:comment xml:lang="en">An UME Squad is a body of soldiers, who belongs to UME (Emergency Military Unit) that make up a unit (as of infantry) consisting usually of two teams. It is commanded by a Sargent or Sargent First Class.</rdfs:comment>
    </owl:Class>
    


    <!-- http://www.semanticweb.org/leopo/ontologies/2022/0/EmergencyAgent#UMETeam -->

    <owl:Class rdf:about="http://www.semanticweb.org/leopo/ontologies/2022/0/EmergencyAgent#UMETeam">
        <rdfs:subClassOf rdf:resource="http://www.semanticweb.org/leopo/ontologies/2022/0/EmergencyAgent#UMEUnit"/>
        <rdfs:comment xml:lang="en">A UME Team is a body of soldiers, who belongs to UME (Emergency Military Unit), that make up a unit (as of infantry) consisting usually of four soldiers. It is commanded by a Corporal.</rdfs:comment>
    </owl:Class>
    


    <!-- http://www.semanticweb.org/leopo/ontologies/2022/0/EmergencyAgent#UMEUnit -->

    <owl:Class rdf:about="http://www.semanticweb.org/leopo/ontologies/2022/0/EmergencyAgent#UMEUnit">
        <rdfs:comment xml:lang="en">UME Unit represent all possible units that Emergency Military Unit has.</rdfs:comment>
    </owl:Class>
    


    <!-- http://www.semanticweb.org/leopo/ontologies/2022/0/EmergencyAgent#Volunteer -->

    <owl:Class rdf:about="http://www.semanticweb.org/leopo/ontologies/2022/0/EmergencyAgent#Volunteer">
        <rdfs:comment xml:lang="en">Volunteer represent citizens that acts individually helping during emergencies.</rdfs:comment>
    </owl:Class>
    


    <!-- http://www.semanticweb.org/leopo/ontologies/2022/0/EmergencyAgent#VolunteerCitizen -->

    <owl:Class rdf:about="http://www.semanticweb.org/leopo/ontologies/2022/0/EmergencyAgent#VolunteerCitizen">
        <rdfs:subClassOf rdf:resource="http://www.semanticweb.org/leopo/ontologies/2022/0/EmergencyAgent#Volunteer"/>
        <rdfs:comment xml:lang="en">A Volunteer is a person who voluntarily undertakes or expresses a willingness to undertake a service.</rdfs:comment>
    </owl:Class>
    


    <!-- http://www.semanticweb.org/leopo/ontologies/2022/0/EmergencyAgent#VolunteerTeam -->

    <owl:Class rdf:about="http://www.semanticweb.org/leopo/ontologies/2022/0/EmergencyAgent#VolunteerTeam">
        <rdfs:subClassOf rdf:resource="http://www.semanticweb.org/leopo/ontologies/2022/0/EmergencyAgent#Volunteer"/>
        <rdfs:comment xml:lang="en">A Volunteer Team is a group of people who voluntarily undertakes or expresses a willingness to undertake a service.</rdfs:comment>
    </owl:Class>
    


    <!-- 
    ///////////////////////////////////////////////////////////////////////////////////////
    //
    // General axioms
    //
    ///////////////////////////////////////////////////////////////////////////////////////
     -->

    <rdf:Description>
        <rdf:type rdf:resource="http://www.w3.org/2002/07/owl#AllDisjointClasses"/>
        <owl:members rdf:parseType="Collection">
            <rdf:Description rdf:about="http://www.semanticweb.org/leopo/ontologies/2022/0/EmergencyAgent#ArmedForcesBatallion"/>
            <rdf:Description rdf:about="http://www.semanticweb.org/leopo/ontologies/2022/0/EmergencyAgent#ArmedForcesBrigade"/>
            <rdf:Description rdf:about="http://www.semanticweb.org/leopo/ontologies/2022/0/EmergencyAgent#ArmedForcesCompany"/>
            <rdf:Description rdf:about="http://www.semanticweb.org/leopo/ontologies/2022/0/EmergencyAgent#ArmedForcesFireExtinguiserPlanePilot"/>
            <rdf:Description rdf:about="http://www.semanticweb.org/leopo/ontologies/2022/0/EmergencyAgent#ArmedForcesHelicopterPilot"/>
            <rdf:Description rdf:about="http://www.semanticweb.org/leopo/ontologies/2022/0/EmergencyAgent#ArmedForcesPlatoon"/>
            <rdf:Description rdf:about="http://www.semanticweb.org/leopo/ontologies/2022/0/EmergencyAgent#ArmedForcesSquad"/>
            <rdf:Description rdf:about="http://www.semanticweb.org/leopo/ontologies/2022/0/EmergencyAgent#ArmedForcesTeam"/>
            <rdf:Description rdf:about="http://www.semanticweb.org/leopo/ontologies/2022/0/EmergencyAgent#CBRNAgent"/>
            <rdf:Description rdf:about="http://www.semanticweb.org/leopo/ontologies/2022/0/EmergencyAgent#CBRNArmedForcesAgent"/>
            <rdf:Description rdf:about="http://www.semanticweb.org/leopo/ontologies/2022/0/EmergencyAgent#CBRNArmedForcesBatallion"/>
            <rdf:Description rdf:about="http://www.semanticweb.org/leopo/ontologies/2022/0/EmergencyAgent#CBRNArmedForcesCompany"/>
            <rdf:Description rdf:about="http://www.semanticweb.org/leopo/ontologies/2022/0/EmergencyAgent#CBRNArmedForcesPlatoon"/>
            <rdf:Description rdf:about="http://www.semanticweb.org/leopo/ontologies/2022/0/EmergencyAgent#CBRNArmedForcesSquad"/>
            <rdf:Description rdf:about="http://www.semanticweb.org/leopo/ontologies/2022/0/EmergencyAgent#CBRNArmedForcesTeam"/>
            <rdf:Description rdf:about="http://www.semanticweb.org/leopo/ontologies/2022/0/EmergencyAgent#SignalCorpsAgent"/>
            <rdf:Description rdf:about="http://www.semanticweb.org/leopo/ontologies/2022/0/EmergencyAgent#SignalCorpsSquad"/>
            <rdf:Description rdf:about="http://www.semanticweb.org/leopo/ontologies/2022/0/EmergencyAgent#SignalCorpsTeam"/>
        </owl:members>
    </rdf:Description>
    <rdf:Description>
        <rdf:type rdf:resource="http://www.w3.org/2002/07/owl#AllDisjointClasses"/>
        <owl:members rdf:parseType="Collection">
            <rdf:Description rdf:about="http://www.semanticweb.org/leopo/ontologies/2022/0/EmergencyAgent#ArmedForcesUnit"/>
            <rdf:Description rdf:about="http://www.semanticweb.org/leopo/ontologies/2022/0/EmergencyAgent#BRIFUnit"/>
            <rdf:Description rdf:about="http://www.semanticweb.org/leopo/ontologies/2022/0/EmergencyAgent#FireBrigadeUnit"/>
            <rdf:Description rdf:about="http://www.semanticweb.org/leopo/ontologies/2022/0/EmergencyAgent#GuardiaCivilUnit"/>
            <rdf:Description rdf:about="http://www.semanticweb.org/leopo/ontologies/2022/0/EmergencyAgent#MedicalServices"/>
            <rdf:Description rdf:about="http://www.semanticweb.org/leopo/ontologies/2022/0/EmergencyAgent#PoliceUnit"/>
            <rdf:Description rdf:about="http://www.semanticweb.org/leopo/ontologies/2022/0/EmergencyAgent#RegionalEmergencyUnit"/>
            <rdf:Description rdf:about="http://www.semanticweb.org/leopo/ontologies/2022/0/EmergencyAgent#UMEUnit"/>
            <rdf:Description rdf:about="http://www.semanticweb.org/leopo/ontologies/2022/0/EmergencyAgent#Volunteer"/>
        </owl:members>
    </rdf:Description>
    <rdf:Description>
        <rdf:type rdf:resource="http://www.w3.org/2002/07/owl#AllDisjointClasses"/>
        <owl:members rdf:parseType="Collection">
            <rdf:Description rdf:about="http://www.semanticweb.org/leopo/ontologies/2022/0/EmergencyAgent#ArmedForcesUnit"/>
            <rdf:Description rdf:about="http://www.semanticweb.org/leopo/ontologies/2022/0/EmergencyAgent#FireBrigadeUnit"/>
            <rdf:Description rdf:about="http://www.semanticweb.org/leopo/ontologies/2022/0/EmergencyAgent#GuardiaCivilUnit"/>
            <rdf:Description rdf:about="http://www.semanticweb.org/leopo/ontologies/2022/0/EmergencyAgent#MedicalServices"/>
            <rdf:Description rdf:about="http://www.semanticweb.org/leopo/ontologies/2022/0/EmergencyAgent#PoliceUnit"/>
            <rdf:Description rdf:about="http://www.semanticweb.org/leopo/ontologies/2022/0/EmergencyAgent#UMEUnit"/>
            <rdf:Description rdf:about="http://www.semanticweb.org/leopo/ontologies/2022/0/EmergencyAgent#Volunteer"/>
        </owl:members>
    </rdf:Description>
    <rdf:Description>
        <rdf:type rdf:resource="http://www.w3.org/2002/07/owl#AllDisjointClasses"/>
        <owl:members rdf:parseType="Collection">
            <rdf:Description rdf:about="http://www.semanticweb.org/leopo/ontologies/2022/0/EmergencyAgent#CBRNUMEAgent"/>
            <rdf:Description rdf:about="http://www.semanticweb.org/leopo/ontologies/2022/0/EmergencyAgent#CBRNUMECompany"/>
            <rdf:Description rdf:about="http://www.semanticweb.org/leopo/ontologies/2022/0/EmergencyAgent#CBRNUMEPlatoon"/>
            <rdf:Description rdf:about="http://www.semanticweb.org/leopo/ontologies/2022/0/EmergencyAgent#CBRNUMESquad"/>
            <rdf:Description rdf:about="http://www.semanticweb.org/leopo/ontologies/2022/0/EmergencyAgent#CBRNUMETeam"/>
            <rdf:Description rdf:about="http://www.semanticweb.org/leopo/ontologies/2022/0/EmergencyAgent#UMEBatallion"/>
            <rdf:Description rdf:about="http://www.semanticweb.org/leopo/ontologies/2022/0/EmergencyAgent#UMECompany"/>
            <rdf:Description rdf:about="http://www.semanticweb.org/leopo/ontologies/2022/0/EmergencyAgent#UMEPlatoon"/>
            <rdf:Description rdf:about="http://www.semanticweb.org/leopo/ontologies/2022/0/EmergencyAgent#UMESoldierAgent"/>
            <rdf:Description rdf:about="http://www.semanticweb.org/leopo/ontologies/2022/0/EmergencyAgent#UMESquad"/>
            <rdf:Description rdf:about="http://www.semanticweb.org/leopo/ontologies/2022/0/EmergencyAgent#UMETeam"/>
        </owl:members>
    </rdf:Description>
    <rdf:Description>
        <rdf:type rdf:resource="http://www.w3.org/2002/07/owl#AllDisjointClasses"/>
        <owl:members rdf:parseType="Collection">
            <rdf:Description rdf:about="http://www.semanticweb.org/leopo/ontologies/2022/0/EmergencyAgent#FireBrigadeAgent"/>
            <rdf:Description rdf:about="http://www.semanticweb.org/leopo/ontologies/2022/0/EmergencyAgent#FireBrigadePlatoon"/>
            <rdf:Description rdf:about="http://www.semanticweb.org/leopo/ontologies/2022/0/EmergencyAgent#FireBrigadeSquad"/>
            <rdf:Description rdf:about="http://www.semanticweb.org/leopo/ontologies/2022/0/EmergencyAgent#FireBrigadeTeam"/>
        </owl:members>
    </rdf:Description>
    <rdf:Description>
        <rdf:type rdf:resource="http://www.w3.org/2002/07/owl#AllDisjointClasses"/>
        <owl:members rdf:parseType="Collection">
            <rdf:Description rdf:about="http://www.semanticweb.org/leopo/ontologies/2022/0/EmergencyAgent#GuardiaCivilAgent"/>
            <rdf:Description rdf:about="http://www.semanticweb.org/leopo/ontologies/2022/0/EmergencyAgent#GuardiaCivilCompany"/>
            <rdf:Description rdf:about="http://www.semanticweb.org/leopo/ontologies/2022/0/EmergencyAgent#GuardiaCivilPatrol"/>
            <rdf:Description rdf:about="http://www.semanticweb.org/leopo/ontologies/2022/0/EmergencyAgent#GuardiaCivilPlatoon"/>
            <rdf:Description rdf:about="http://www.semanticweb.org/leopo/ontologies/2022/0/EmergencyAgent#GuardiaCivilSquad"/>
            <rdf:Description rdf:about="http://www.semanticweb.org/leopo/ontologies/2022/0/EmergencyAgent#GuardiaCivilTeam"/>
        </owl:members>
    </rdf:Description>
</rdf:RDF>



<!-- Generated by the OWL API (version 4.5.9.2019-02-01T07:24:44Z) https://github.com/owlcs/owlapi -->

